lambda.agda
@@ -1,0 +1,246 @@
+-- Basic
+data ⊥ : Set where
+data ⊤ : Set where
+  tt : ⊤
+data _⊎_ (A : Set) (B : Set) : Set where
+  inj₁ : (x : A) → A ⊎ B
+  inj₂ : (y : B) → A ⊎ B
+data ∃ {A} (P : A → Set) : Set where
+  _,_ : ∀ x → P x → ∃ P
+
+¬_ : Set → Set
+¬ A = A → ⊥
+data Dec (P : Set) : Set where
+  yes : P → Dec P
+  no  : ¬ P → Dec P
+
+data _≡_ {a} {A : Set a} (x : A) : A → Set a where
+  instance refl : x ≡ x
+sym : ∀ {A : Set} {x y : A} → x ≡ y → y ≡ x
+sym refl = refl
+trans : ∀ {A : Set} {x y z : A} → x ≡ y → y ≡ z → x ≡ z
+trans refl refl = refl
+cong : ∀ {A B : Set} {x y : A} → (f : A → B) → x ≡ y → f x ≡ f y
+cong f refl = refl
+
+⊥-elim : ∀ {A : Set} → ⊥ → A
+⊥-elim ()
+_≠_ : ∀ {A : Set} → A → A → Set
+x ≠ y = ¬ (x ≡ y)
+≠-refl : ∀ {A B} {x : A} → x ≠ x → B
+≠-refl eq = ⊥-elim (eq refl)
+≠-sym : ∀ {A} {x y : A} → x ≠ y → y ≠ x
+≠-sym neq eq = neq (sym eq)
+
+data ℕ : Set where
+  zero : ℕ
+  suc  : ℕ → ℕ
+_≟_ : ∀ (x y : ℕ) → Dec (x ≡ y)
+zero ≟ zero = yes refl
+zero ≟ suc y = no (λ())
+suc x ≟ zero = no (λ())
+suc x ≟ suc y with x ≟ y
+... | yes refl = yes refl
+... | no neq = no (λ x1 → neq (neq2 x1))
+  where
+    neq2 : suc x ≡ suc y → x ≡ y
+    neq2 refl = refl
+
+Id : Set
+Id = ℕ
+
+infixr 7 _⇒_
+
+data Type : Set where
+  `bool                   :  Type
+  _⇒_                     :  Type → Type → Type
+
+infix  5  ƛ_⦂_⇒_
+infixl 7  _·_
+infix  8  `if_then_else_
+infix  9  `_
+
+data Term : Set where
+  `_                      :  Id → Term
+  ƛ_⦂_⇒_                  :  Id -> Type → Term → Term
+  _·_                     :  Term → Term → Term
+  `true                   :  Term
+  `false                  :  Term
+  `if_then_else_          :  Term → Term → Term → Term
+
+data Value : Term → Set where
+  V-ƛ : ∀ {x T t} → Value (ƛ x ⦂ T ⇒ t)
+  V-true : Value `true
+  V-false : Value `false
+
+infix 9 _[_:=_]
+
+_[_:=_] : Term → Id → Term → Term
+(` x) [ y := V ] with x ≟ y
+... | yes _ = V
+... | no _ = ` x
+(ƛ x ⦂ T ⇒ t) [ y := V ] with x ≟ y
+... | yes _ = ƛ x ⦂ T ⇒ t
+... | no _ = ƛ x ⦂ T ⇒ (t [ y := V ])
+(L · R) [ y := V ] = (L [ y := V ]) · (R [ y := V ])
+`true [ y := V ] = `true
+`false [ y := V ] = `false
+(`if C then T else E) [ y := V ] = `if (C [ y := V ]) then (T [ y := V ]) else (E [ y := V ])
+
+infix 4 _—→_
+
+data _—→_ : Term → Term → Set where
+  ξ-·₁ : ∀ {L L′ M}
+    → L —→ L′
+    → L · M —→ L′ · M
+  ξ-·₂ : ∀ {V M M′}
+    → Value V
+    → M —→ M′
+    → V · M —→ V · M′
+  β-· : ∀ {x T N V}
+    → Value V
+    → (ƛ x ⦂ T ⇒ N) · V —→ N [ x := V ]
+
+  ξ-if : ∀ {L L′ M N}
+    → L —→ L′
+    → `if L then M else N —→ `if L′ then M else N
+  β-if-true : ∀ {M N}
+    → `if `true then M else N —→ M
+  β-if-false : ∀ {M N}
+    → `if `false then M else N —→ N
+
+Context : Set
+Context = Id → (Type ⊎ ⊤)
+
+infixl 5 _,_⦂_
+_,_⦂_ : Context → Id → Type → Context
+(Γ , x ⦂ T) y with y ≟ x
+...| yes _ = inj₁ T
+...| no  _ = Γ y
+
+infix 4 _⊢_⦂_
+data _⊢_⦂_ : Context → Term → Type → Set where
+  ⊢` : ∀ {Γ x T}
+    → Γ x ≡ inj₁ T
+    → Γ ⊢ ` x ⦂ T
+  ⊢ƛ : ∀ {Γ x T t U}
+    → Γ , x ⦂ T ⊢ t ⦂ U
+    → Γ ⊢ ƛ x ⦂ T ⇒ t ⦂ T ⇒ U
+  ⊢· : ∀ {Γ L M T U}
+    → Γ ⊢ L ⦂ T ⇒ U
+    → Γ ⊢ M ⦂ T
+    → Γ ⊢ L · M ⦂ U
+  ⊢true : ∀ {Γ}
+    → Γ ⊢ `true ⦂ `bool
+  ⊢false : ∀ {Γ}
+    → Γ ⊢ `false ⦂ `bool
+  ⊢if : ∀ {Γ L M N T}
+    → Γ ⊢ L ⦂ `bool
+    → Γ ⊢ M ⦂ T
+    → Γ ⊢ N ⦂ T
+    → Γ ⊢ `if L then M else N ⦂ T
+
+empty : Context
+empty x = inj₂ tt
+
+data Progress (M : Term) : Set where
+  step : ∀ {N}
+    → M —→ N
+    → Progress M
+  done :
+      Value M
+      ----------
+    → Progress M
+
+progress : ∀ {M T}
+  → empty ⊢ M ⦂ T
+  → Value M ⊎ ∃ (λ M′ → M —→ M′)
+progress (⊢ƛ ⊢N) = inj₁ V-ƛ
+progress (⊢· ⊢L ⊢M) with progress ⊢L
+... | inj₂ ( _ , S ) = inj₂ ( _ , (ξ-·₁ S) )
+... | inj₁ V-ƛ with progress ⊢M
+...   | inj₂ ( _ , S ) = inj₂ ( _ , (ξ-·₂ V-ƛ S) )
+...   | inj₁ VM = inj₂ ( _ , (β-· VM) )
+progress ⊢true = inj₁ V-true
+progress ⊢false = inj₁ V-false
+progress (⊢if C T F) with progress C
+... | inj₂ ( _ , S ) = inj₂ ( _ , (ξ-if S) )
+... | inj₁ V-true = inj₂ ( _ , β-if-true )
+... | inj₁ V-false = inj₂ ( _ , β-if-false )
+
+map≡ : Context → Context → Set
+map≡ Γ Γ′ = ∀ x → Γ x ≡ Γ′ x
+
+upd≡ : ∀ {Γ Γ′ x T} → map≡ Γ Γ′ → map≡ (Γ , x ⦂ T) (Γ′ , x ⦂ T)
+upd≡ {_} {_} {x} equ y with y ≟ x
+... | yes refl = refl
+... | no _ = equ y
+
+shadow≡ : ∀ {Γ x v1 v2} → map≡ (Γ , x ⦂ v1 , x ⦂ v2) (Γ , x ⦂ v2)
+shadow≡ {Γ} {y} {v1} {v2} x with x ≟ y
+shadow≡ {Γ} {y} {v1} {v2} x | yes refl = refl
+shadow≡ {Γ} {y} {v1} {v2} x | no _ with x ≟ y
+shadow≡ {Γ} {y} {v1} {v2} x | no neq | yes refl = ≠-refl neq
+shadow≡ {Γ} {y} {v1} {v2} x | no _ | no _ = refl
+
+permute≡ : ∀ {Γ x y} → (x ≡ y → ⊥) → ∀ {v1 v2} → map≡ (Γ , x ⦂ v1 , y ⦂ v2) (Γ , y ⦂ v2 , x ⦂ v1)
+permute≡ {_} {x} {y} neq z with z ≟ x | z ≟ y
+permute≡ {_} {x} {y} neq z | yes refl | yes refl = ≠-refl neq
+permute≡ {_} {x} {y} neq z | yes refl | no neq2 with x ≟ x
+permute≡ {_} {x} {y} neq z | yes refl | no neq2 | yes _ = refl
+permute≡ {_} {x} {y} neq z | yes refl | no neq2 | no neq1 = ≠-refl neq1
+permute≡ {_} {x} {y} neq z | no neq1 | yes refl with y ≟ y
+permute≡ {_} {x} {y} neq z | no neq1 | yes refl | yes _ = refl
+permute≡ {_} {x} {y} neq z | no neq1 | yes refl | no neq2 = ≠-refl neq2
+permute≡ {_} {x} {y} neq z | no neq1 | no neq2 with z ≟ x | z ≟ y
+permute≡ {_} {x} {y} neq z | no neq1 | no neq2 | yes refl | _ = ≠-refl neq1
+permute≡ {_} {x} {y} neq z | no neq1 | no neq2 | no neq3  | yes refl = ≠-refl neq2
+permute≡ {_} {x} {y} neq z | no neq1 | no neq2 | no neq3  | no neq4 = refl
+
+_⊆_ : Context → Context → Set
+Γ ⊆ Γ′ = ∀ x v → Γ x ≡ inj₁ v → Γ′ x ≡ inj₁ v
+
+⊆-update : ∀ {Γ Γ′ x T} → Γ ⊆ Γ′ → (Γ , x ⦂ T) ⊆ (Γ′ , x ⦂ T)
+⊆-update {_} {_} {x} ⊆ y v eq with y ≟ x
+⊆-update {_} {_} {x} ⊆ y v eq | yes _ = eq
+⊆-update {_} {_} {x} ⊆ y v eq | no _ = ⊆ y v eq
+
+weak : ∀ {Γ Γ'} → Γ ⊆ Γ' → ∀ {t} {T} → Γ ⊢ t ⦂ T → Γ' ⊢ t ⦂ T
+weak {Γ} {Γ'} ⊆Γ (⊢` x) = ⊢` (⊆Γ _ _ x)
+weak {Γ} {Γ'} ⊆Γ (⊢ƛ ⊢) = ⊢ƛ (weak (⊆-update ⊆Γ) ⊢)
+weak {Γ} {Γ'} ⊆Γ (⊢· ⊢ ⊢₁) = ⊢· (weak ⊆Γ ⊢) (weak ⊆Γ ⊢₁)
+weak {Γ} {Γ'} ⊆Γ ⊢true = ⊢true
+weak {Γ} {Γ'} ⊆Γ ⊢false = ⊢false
+weak {Γ} {Γ'} ⊆Γ (⊢if ⊢ ⊢₁ ⊢₂) = ⊢if (weak ⊆Γ ⊢) (weak ⊆Γ ⊢₁) (weak ⊆Γ ⊢₂)
+
+⊂-refl : ∀ {Γ Γ'} → (map≡ Γ Γ') → (Γ ⊆ Γ')
+⊂-refl equ x v eq = trans (sym (equ x)) eq
+
+cong≡ : ∀ {Γ Γ′} → map≡ Γ Γ′ → ∀ {t} {T} → Γ ⊢ t ⦂ T → Γ′ ⊢ t ⦂ T
+cong≡ equ ⊢ = weak (⊂-refl equ) ⊢
+
+weak-∅ : ∀ {Γ} → ∀ {t} {T} → empty ⊢ t ⦂ T → Γ ⊢ t ⦂ T
+weak-∅ {Γ} ⊢ = weak (λ x v ()) ⊢
+
+subst⊢ : ∀ {Γ x T t U V}
+  → empty ⊢ V ⦂ T
+  → Γ , x ⦂ T ⊢ t ⦂ U
+  → Γ ⊢ t [ x := V ] ⦂ U
+subst⊢ {_} {x} ⊢V (⊢` {_} {y} ∈) with y ≟ x
+subst⊢ {_} {x} ⊢V (⊢` {_} {y} refl) | yes refl = weak-∅ ⊢V
+subst⊢ {_} {x} ⊢V (⊢` {_} {y} ∈) | no _ = ⊢` ∈
+subst⊢ {_} {x} ⊢V (⊢ƛ {_} {y} ⊢t) with y ≟ x | ⊢t
+subst⊢ ⊢V (⊢ƛ ⊢t) | yes refl | _ = ⊢ƛ (cong≡ shadow≡ ⊢t)
+subst⊢ {Γ} ⊢V (⊢ƛ ⊢t) | no neq     | _ = ⊢ƛ (subst⊢ ⊢V (cong≡ (permute≡ (≠-sym neq)) ⊢t))
+subst⊢ ⊢V (⊢· ⊢t ⊢t₁) = ⊢· (subst⊢ ⊢V ⊢t) (subst⊢ ⊢V ⊢t₁)
+subst⊢ ⊢V ⊢true = ⊢true
+subst⊢ ⊢V ⊢false = ⊢false
+subst⊢ ⊢V (⊢if ⊢t ⊢t₁ ⊢t₂) = ⊢if (subst⊢ ⊢V ⊢t) (subst⊢ ⊢V ⊢t₁) (subst⊢ ⊢V ⊢t₂)
+
+preserve : ∀ {t t' T} → empty ⊢ t ⦂ T → t —→ t' → empty ⊢ t' ⦂ T
+preserve (⊢· ⊢ ⊢₁) (ξ-·₁ ——) = ⊢· (preserve ⊢ ——) ⊢₁
+preserve (⊢· ⊢ ⊢₁) (ξ-·₂ x ——) = ⊢· ⊢ (preserve ⊢₁ ——)
+preserve (⊢· (⊢ƛ ⊢) ⊢₁) (β-· x) = subst⊢ ⊢₁ ⊢
+preserve (⊢if ⊢ ⊢₁ ⊢₂) (ξ-if ——) = ⊢if (preserve ⊢ ——) ⊢₁ ⊢₂
+preserve (⊢if ⊢ ⊢₁ ⊢₂) β-if-true = ⊢₁
+preserve (⊢if ⊢ ⊢₁ ⊢₂) β-if-false = ⊢₂
